\documentclass[12pt]{article}
\usepackage[english]{babel}
\usepackage[utf8]{inputenc}
\usepackage{amsmath, amssymb,amsthm}
\usepackage{graphicx}
\usepackage{hyperref}
\usepackage{geometry}

\setlength{\topmargin}{0pt}
\setlength{\headsep}{0pt}
\textheight = 600pt

\title{Real Analysis \\ Homework 15}
\author{Ben Kallus, Noah Barton}
\date{Due Thursday, October 22}

\begin{document}
\maketitle

\hrule
\bigskip

\noindent {\bf Acknowledgements:} None.

\bigskip
\hrule
\bigskip

\noindent{\bf 26. Claim:} If $a_n > 0$ and $b_n > 0$ for every $n \in \mathbb N$, and $\lim\limits_{n\to\infty}\frac{a_n}{b_n}=c$, where $c > 0$, then $\sum\limits_{n=1}^\infty a_n$ converges if and only if $\sum\limits_{n=1}^\infty b_n$ converges.
\begin{proof}
    Since $\lim\limits_{n\to\infty}\frac{a_n}{b_n} = c$, there exists $N$ such that for all $n \geq N$, $\left|\frac{a_n}{b_n} - c\right| < \frac c2$. Thus, $\frac c2 < \frac{a_n}{b_n} < \frac{3c}2$ for all $n \geq N$. Thus, $\frac c2 b_n < a_n < \frac{3c}2 b_n$ for all $n \in \mathbb N$. Therefore, $b_n < \frac 2c a_n$ and $a_n < \frac{3c}2 b_n$ for all $n \in \mathbb N$. Suppose $\sum\limits_{n=1}^\infty a_n$ converges. Then, by the Algebraic Limit Theorem for series, $\sum\limits_{n=1}^\infty \frac2c\frac{a_n}{b_n}$ converges. Thus, by the Comparison Test, $\sum\limits_{n=1}^\infty b_n$ converges. Now, suppose $\sum\limits_{n=1}^\infty b_n$ converges. Then, by the Algebraic Limit Theorem for series, $\sum\limits_{n=1}^\infty \frac{3c}2 b_n$ converges. Thus, by the Comparison Test, $\sum\limits_{n=1}^\infty a_n$ converges. Thus, $\sum\limits_{n=1}^\infty a_n$ converges if and only if $\sum\limits_{n=1}^\infty b_n$ converges.
\end{proof}

\newpage
\noindent{\bf 27.}

\noindent{\bf a. Claim:} The series $\sum\limits_{n=1}^\infty \frac{n+3}{n+4}$ diverges.
\begin{proof}
    Observe that for all $n \in \mathbb N$,
    \begin{align*}
        \frac{n+3}{n+4} &> \frac{n+3}{2n+6} \\
                        &= \frac12.
    \end{align*}
    Define the series $(a_n)$ by $a_n = \frac1{n+1}$. Note that $(a_n)$ is the harmonic sequence without the first term. Thus, $\sum\limits_{n=1}^\infty a_n$ diverges. Since $(a_n)$ is decreasing, all of its terms are less than or equal to $a_1 = \frac12$. Thus, by the Comparison Test, $\sum\limits_{n=1}^\infty \frac{n+3}{n+4}$ diverges.
\end{proof}

\newpage
\noindent{\bf b. Claim:} The series $\sum\limits_{n=1}^\infty \frac{n+3^n}{n+4^n}$ converges.
\begin{proof}
    Observe that for all $n \in \mathbb N$,
    \begin{align*}
        \frac{n+3^n}{n+4^n} &\leq \frac{n+3^n}{4^n} \\
                            &= \frac n{4^n} + \frac{3^n}{4^n} \\
                            &= \frac n{4^n} + \left(\frac34\right)^n.
    \end{align*}
    Since $\sum\limits_{n=1}^\infty \left(\frac34\right)^n$ is a convergent geometric series, we have that if $\sum\limits_{n=1}^\infty\frac{n}{4^n}$ converges, then $\sum\limits_{n=1}^\infty \frac{n+3^n}{n+4^n}$ converges.
    
    Toward this end, we first show that $\frac1{4^n} < \frac1{n^3}$ for all $n \in \mathbb N$. Note that for all $n \geq 3$,
    \begin{align*}
        n^3 &= n \cdot n \cdot n \\
            &\geq 3 \cdot n \cdot n \\
            &= 3n^2 \\
            &> 3n.
    \end{align*} Thus, $n^3 > 3n^2$ and $n^3 > 3n$ for all $n \geq 3$.
    
    For the base cases, observe that $\frac1{4^n} < \frac1{n^3}$ for $n \in \{1,2\}$. Begin the inductive step by assuming that there exists $n$ such that $\frac1{4^{n}} < \frac1{n^3}$. Then,
    \begin{align*}
        \frac1{4^{n+1}} &< \frac1{4n^3} \\
                        &= \frac1{n^3 + n^3 + n^3 + n^3} \\
                        &< \frac1{n^3 + 3n^2 + 3n + 1} \\
                        &= \frac1{(n+1)^3}.
    \end{align*} Thus, by the Principle of Mathematical Induction, $\frac1{4^n} < \frac1{n^3}$ for all $n \in \mathbb N$. Then, $\frac n {4^n} < \frac n {n^3} = \frac 1 {n^2}$ for all $n \in \mathbb N$. Thus, since $\sum\limits_{n=1}^\infty \frac1{n^2}$ is convergent, $\sum\limits_{n=1}^\infty \frac n {4^n}$ must be convergent by the Comparison Test. Therefore, by the Algebraic Limit Theorem for series, $\sum\limits_{n=1}^\infty \frac n{4^n} + \left(\frac34\right)^n$ converges. Thus, by the Comparison Test, $\sum\limits_{n=1}^\infty \frac{n+3^n}{n+4^n}$ converges.
\end{proof}

\newpage
\noindent{\bf 28.} Let $\sum\limits_{n=1}^\infty a_n$ be a convergent series, and let $(b_n)$ be a bounded sequence, with $a_n \geq 0$ and $b_n \geq 0$ for every $n \in \mathbb N$.

\medskip
\noindent{\bf a. Claim:} The series $\sum\limits_{n=1}^\infty a_n b_n$ converges.
\begin{proof}
    Since $(b_n)$ is bounded and all nonnegative, there exists $M > 0$ such that $b_n \leq M$ for all $n \in \mathbb N$. Then, by the Algebraic Limit Theorem for series, $\sum\limits_{n=1}^\infty a_n \cdot M$ converges. Observe that $$\sum\limits_{n=1}^\infty a_n \cdot M \geq \sum\limits_{n=1}^\infty a_n \cdot b_n.$$ Thus, by the Comparison Test, $\sum\limits_{n=1}^\infty a_n b_n$ converges.
\end{proof}

\medskip
\noindent{\bf b. Claim:} The series $\sum\limits_{n=1}^\infty a_n b_n$ converges.
\begin{proof}
    Let $\epsilon > 0$ be given. Since $(b_n)$ is bounded and all nonnegative, there exists $M > 0$ such that $b_n \leq M$ for all $n \in \mathbb N$. Then, by the Cauchy Criterion for series, there exists $N \in \mathbb N$ such that for all $n,m \geq N$, with $n > m$, $|a_{m+1} + \hdots + a_n| < \frac\epsilon M$. Observe that for all $n,m \geq N$ with $n > m$,
    \begin{align*}
        |a_{m+1}b_{m+1} + \hdots + a_n b_n| &= |a_{m+1}b_{m+1} + \hdots + a_n b_n| \\
                                            &\leq |a_{m+1}M + \hdots + a_nM| \\
                                            &= M|a_{m+1} + \hdots a_n| \\
                                            &< M\left(\frac\epsilon M\right) \\
                                            &= \epsilon.
    \end{align*} Thus, by the Cauchy Criterion for series, $\sum\limits_{n=1}^\infty a_n b_n$ converges.
\end{proof}
    
\end{document}