\documentclass[12pt]{article}
\usepackage[english]{babel}
\usepackage[utf8]{inputenc}
\usepackage{amsmath, amssymb,amsthm}
\usepackage{graphicx}
\usepackage{hyperref}
\usepackage{geometry}
\usepackage{xcolor}

\setlength{\topmargin}{0pt}
\setlength{\headsep}{0pt}
\textheight = 600pt

\title{Real Analysis \\ Homework 19}
\author{Ben Kallus and Jonathan Sills}
\date{Due Thursday, November 5, 2020}

\begin{document}
\pagecolor{black}
\color{white}
\maketitle

\hrule
\bigskip

\noindent {\bf Acknowledgements:} 

\bigskip
\hrule
\bigskip

\noindent{\bf 2.} Let $f$ and $g$ be functions defined on a domain $A \subseteq \mathbb R$ such that for some limit point $c$ in $A$, $\lim\limits_{x\to c}f(x)=L$ and $\lim\limits_{x\to c}g(x) = M$.

\medskip
\noindent{\bf a.} Claim: $\lim\limits_{x \to c}[f(x) + g(x)] = L + M$.
\begin{proof}
    Let $\epsilon > 0$ be given.
    Then, since $\lim\limits_{x\to c}f(x)=L$, there exists $\delta_f$ such that for all $x \in A$ satisfying $0 < |x - c| < \delta_f$, $|f(x) - L| < \frac\epsilon2$.
    Similarly, since $\lim\limits_{x\to c}g(x)=L$, there exists $\delta_g$ such that  for all $x \in A$ satisfying $0 < |x - c| < \delta_g$, $|g(x) - M| < \frac\epsilon2$.
    Define $\delta = \min\{\delta_f, \delta_g\}$.
    Then, for all $x \in A$ satisfying $0 < |x - c| < \delta$, $|f(x) - L| < \frac\epsilon2$ and $|g(x) - M| < \frac\epsilon2$.
    Thus, $|f(x) - L| + |g(x) - M| < \epsilon$.
    Therefore, $|f(x) - L + g(x) - M| < \epsilon$.
    Then, $|(f(x) - g(x)) - (L + M)| < \epsilon$.
    Thus, $\lim\limits_{x \to c}[f(x) + g(x)] = L + M$.
\end{proof}

\medskip
\noindent{\bf b.} Claim: $\lim\limits_{x \to c}[f(x) + g(x)] = L + M$.
\begin{proof}
    Let $(x_n)$ be a sequence in $A$ such that $(x_n) \to c$ and $x_n \neq c$ for all $n \in \mathbb N$.
    Then, by Theorem 4.2.3, since $\lim\limits_{x\to c}f(x)=L$, $\lim\limits_{n\to \infty}f(x_n) = L$.
    Similarly, since $\lim\limits_{x\to c}g(x)=L$, $\lim\limits_{n\to \infty}g(x_n) = M$.
    Then, by the algebraic limit theorem for sequences, $\lim\limits_{n\to \infty}[f(x_n) + g(x_n)] = L + M$.
    Thus, by Theorem 4.2.3, $\lim\limits_{x \to c}[f(x) + g(x)] = L + M$.
\end{proof}

\newpage
\noindent{\bf 3.} Let $A \subseteq \mathbb R$, and let $f:A \to \mathbb R$, $g: A \to \mathbb R$. If there exists $M$ such that $|g(x)| \leq M$ for all $x \in A$, and for some limit point $c$ in $A$, $\lim\limits_{x \to c} f(x) = 0$, then $\lim\limits_{x \to c}f(x)g(x) = 0$.
\begin{proof}
    Let $\epsilon > 0$ be given.
    Suppose there exists $M>0$ such that $|g(x)|\leq M$ for all $x \in A$, and that $\lim\limits_{x \to c} f(x) = 0$ for some limit point $c$ in $A$. 
    Then, there exists $\delta$ such that for all $x \in A$ satisfying $0 < |x -c| < \delta$, $|f(x) - 0| < \frac\epsilon M$.
    Observe that
    \begin{align*}
        |f(x)g(x) - 0| &= |f(x)| \cdot |g(x)| \\
                       &\leq |f(x) - 0| \cdot M \\
                       &< \frac\epsilon M \cdot M \\
                       &= \epsilon.
    \end{align*}
    Thus, $\lim\limits_{x \to c}f(x)g(x) = 0$.
\end{proof}


\newpage
\noindent{\bf 4.}

\medskip
\noindent{\bf a.} Claim: $\lim\limits_{x \to 4} \sqrt x = 2$.
\begin{proof}
    Let $\epsilon > 0$ be given.
    Let $\delta = \min\{1, \epsilon(\sqrt3 + 2)\}$.
    Suppose $0 < |x - 4| < \delta$.
    Then, since $\delta \leq 1$, $3 < x$, so $\sqrt3 + 2 < \sqrt x + 2$.
    Then,
    \begin{align*}
        |\sqrt x - 2| &= \frac{|x - 4|}{|\sqrt x + 2|} \\
                      &< \frac{\epsilon(\sqrt3 + 2)}{|\sqrt x + 2|} \\
                      &< \frac{\epsilon(\sqrt3 + 2)}{\sqrt3 + 2} \\
                      &= \epsilon.
    \end{align*}
    Thus, $\lim\limits_{x \to 4} \sqrt x = 2$.
\end{proof}

\medskip
\noindent{\bf b.} Claim: $\lim\limits_{x \to 4} \sqrt x = 2$.
\begin{proof}
    Let $(x_n)$ be a sequence in $\mathbb R$ such that $\lim\limits_{x \to \infty} x_n = 4$ and $x_n \neq 4$ for all $n \in \mathbb N$. By the result of Problem 15 of Chapter 2, $\lim\limits_{n \to \infty} \sqrt{x_n} = \sqrt4 = 2$. Thus, by Theorem 4.2.3, $\lim\limits_{x\to4} \sqrt x = 2$.
\end{proof}

\end{document}